access-control, infoflow: use generic relation for pasDomainAbs
This patch generalises the mapping between authority labels and
scheduler domains, so that the access-control integrity property still
holds when labels are not partitioned into domains. This lets us use
the integrity result on systems that don't use the domain scheduler.

The information flow proofs still rely on the domain partitioning,
hence we add constraints on the label-domain mapping for the info-flow
results to hold.

Jira VER-945

proof/infoflow/InfoFlow.thy
@@ -27,6 +27,44 @@ begin
 
 context begin interpretation Arch . (*FIXME: arch_split*)
 
+section {* Scheduler domain constraint *}
+
+text {*
+  For the information flow theorem, we assume that every domain
+  contains threads of exactly one label, so that labels cannot leak
+  information through the scheduler.
+
+  Morally, domains that have no labels ought to be allowed as well,
+  but this definition is easier to reason about. In practice, we can
+  just put all empty domains into some dummy label to satisfy the
+  exactly-one requirement. See e.g. the mapping in Example_Valid_State.
+*}
+
+definition pas_domains_distinct :: "('a, 'b) PAS_scheme \<Rightarrow> bool"
+  where
+    "pas_domains_distinct aag \<equiv> \<forall>d. \<exists>l. pasDomainAbs aag d = {l}"
+
+lemma pas_domains_distinct_inj:
+  "\<lbrakk> pas_domains_distinct aag;
+     l1 \<in> pasDomainAbs aag d;
+     l2 \<in> pasDomainAbs aag d \<rbrakk> \<Longrightarrow>
+   l1 = l2"
+  apply (clarsimp simp: pas_domains_distinct_def)
+  apply (drule_tac x=d in spec)
+  apply auto
+  done
+
+lemma domain_has_unique_label:
+  "pas_domains_distinct aag \<Longrightarrow> \<exists>l. pasDomainAbs aag d = {l}"
+  by (simp add: pas_domains_distinct_def)
+
+lemma domain_has_the_label:
+  "pas_domains_distinct aag \<Longrightarrow> l \<in> pasDomainAbs aag d \<Longrightarrow> the_elem (pasDomainAbs aag d) = l"
+  apply (simp add: pas_domains_distinct_def)
+  apply (metis singletonD the_elem_eq)
+  done
+
+
 section {* Reading: subjectReads and associated equivalence properties *}
 
 subsection {* subjectReads *}
@@ -137,9 +175,12 @@ abbreviation aag_can_read_asid :: "'a PAS \<Rightarrow> asid \<Rightarrow> bool"
 where
   "aag_can_read_asid aag x \<equiv> (pasASIDAbs aag x) \<in> subjectReads (pasPolicy aag) (pasSubject aag)"
 
+(* FIXME: having an op\<noteq> in the definition causes clarsimp to spuriously
+   apply classical rules. Using @{term disjnt} may avoid this issue *)
 abbreviation aag_can_read_domain :: "'a PAS \<Rightarrow> domain \<Rightarrow> bool"
 where
-  "aag_can_read_domain aag x \<equiv> (pasDomainAbs aag x) \<in> subjectReads (pasPolicy aag) (pasSubject aag)"
+  "aag_can_read_domain aag x \<equiv>
+     pasDomainAbs aag x \<inter> subjectReads (pasPolicy aag) (pasSubject aag) \<noteq> {}"
 
 lemma aag_can_read_self:
   "is_subject aag x \<Longrightarrow> aag_can_read aag x"
@@ -350,7 +391,15 @@ abbreviation states_equiv_for_labels :: "'a PAS \<Rightarrow> ('a \<Rightarrow> 
 where
   "states_equiv_for_labels aag P \<equiv>
       states_equiv_for (\<lambda> x. P (pasObjectAbs aag x)) (\<lambda> x. P (pasIRQAbs aag x))
-                       (\<lambda> x. P (pasASIDAbs aag x))   (\<lambda> x. P (pasDomainAbs aag x))"
+                       (\<lambda> x. P (pasASIDAbs aag x))   (\<lambda> x. \<exists>l\<in>pasDomainAbs aag x. P l)"
+
+(* We need this to correctly complement the domain mapping, i.e. it's not true that
+     states_equiv_but_for_labels aag P = states_equiv_for_labels aag (not P) *)
+abbreviation states_equiv_but_for_labels :: "'a PAS \<Rightarrow> ('a \<Rightarrow> bool)\<Rightarrow> det_state \<Rightarrow> det_state \<Rightarrow> bool"
+where
+  "states_equiv_but_for_labels aag P \<equiv>
+      states_equiv_for (\<lambda> x. \<not> P (pasObjectAbs aag x)) (\<lambda> x. \<not> P (pasIRQAbs aag x))
+                       (\<lambda> x. \<not> P (pasASIDAbs aag x))   (\<lambda> x. \<forall>l\<in>pasDomainAbs aag x. \<not> P l)"
 
 lemma states_equiv_forI:
   "\<lbrakk>equiv_for P kheap s s';
@@ -846,13 +895,15 @@ where
 abbreviation aag_can_affect_domain
 where
   "aag_can_affect_domain aag l \<equiv> \<lambda>x. aag_can_affect_label aag l \<and>
-                                      pasDomainAbs aag x \<in> subjectReads (pasPolicy aag) l"
+                                      pasDomainAbs aag x \<inter> subjectReads (pasPolicy aag) l \<noteq> {}"
 
 
 lemma affects_equiv_def2:
   "affects_equiv aag l s s' = states_equiv_for (aag_can_affect aag l) (aag_can_affect_irq aag l) (aag_can_affect_asid aag l) (aag_can_affect_domain aag l) s s'"
   apply(clarsimp simp: affects_equiv_def)
-  apply(auto intro!: states_equiv_forI equiv_for_trivial equiv_asids_trivial elim: states_equiv_forE)
+  apply(auto intro!: states_equiv_forI equiv_forI equiv_asids_trivial
+             dest: equiv_forD
+             elim!: states_equiv_forE)
   done
 
 lemma affects_equivE:
@@ -1142,7 +1193,7 @@ lemma states_equiv_for_guard_imp:
 lemma cur_subject_reads_equiv_affects_equiv:
   "pasSubject aag = l \<Longrightarrow>
    reads_equiv aag s s' \<Longrightarrow> affects_equiv aag l s s'"
-  apply(clarsimp simp: reads_equiv_def2 affects_equiv_def simp: states_equiv_for_def)
+  apply(auto simp: reads_equiv_def2 affects_equiv_def equiv_for_def states_equiv_for_def)
   done
 
 (* This lemma says that, if we prove reads_respects above for all l, we will
@@ -1332,14 +1383,20 @@ lemma gets_is_original_cap_revrv':
   apply(fastforce simp: equiv_for_comp[symmetric] equiv_for_or or_comp_dist elim: reads_equivE)
   done
 
+(* FIXME: MOVE *)
+lemma intersection_empty:
+  "(A \<inter> B = {}) = (\<not>(\<exists>x. x \<in> A \<and> x \<in> B))"
+  by blast
+
 lemma gets_ready_queues_revrv:
   "reads_equiv_valid_rv_inv (affects_equiv aag l) aag
                             (equiv_for (aag_can_read_domain aag or aag_can_affect_domain aag l) id)
                             \<top> (gets ready_queues)"
   apply(rule equiv_valid_rv_guard_imp)
    apply(rule gets_evrv)
-  apply(fastforce simp: equiv_for_comp[symmetric] equiv_for_or or_comp_dist equiv_for_def
-                  elim: reads_equivE affects_equivE)
+  (* NB: only clarsimp works here *)
+  apply(clarsimp simp: equiv_for_comp[symmetric] equiv_for_or or_comp_dist equiv_for_def intersection_empty
+                 elim!: reads_equivE affects_equivE)
   done
 
 
@@ -1347,7 +1404,9 @@ lemma gets_ready_queues_revrv':
   "reads_equiv_valid_rv_inv A aag (equiv_for (aag_can_read_domain aag) id) \<top> (gets ready_queues)"
   apply(rule equiv_valid_rv_guard_imp)
    apply(rule gets_evrv)
-  apply(fastforce simp: equiv_for_comp[symmetric] equiv_for_or or_comp_dist equiv_for_def elim: reads_equivE)
+  (* NB: only force works here *)
+  apply(force simp: equiv_for_comp[symmetric] equiv_for_or or_comp_dist equiv_for_def intersection_empty
+              elim: reads_equivE)
   done
 
 
@@ -1657,7 +1716,7 @@ section {* Constraining modifications to a set of label *}
 definition equiv_but_for_labels
 where
   "equiv_but_for_labels aag L s s' \<equiv>
-      states_equiv_for_labels aag (\<lambda>l. l \<notin> L) s s' \<and>
+      states_equiv_but_for_labels aag (\<lambda>l. l \<in> L) s s' \<and>
       cur_thread s = cur_thread s' \<and> cur_domain s = cur_domain s' \<and>
       scheduler_action s = scheduler_action s' \<and> work_units_completed s = work_units_completed s' \<and>
       equiv_irq_state (machine_state s) (machine_state s')"
